DeBruijnSSA.lean
@@ -1,3 +1,5 @@
 import DeBruijnSSA.BinSyntax.Syntax
 import DeBruijnSSA.BinSyntax.Typing
 import DeBruijnSSA.BinSyntax.Subst
+import DeBruijnSSA.BinSyntax.Compose
+import DeBruijnSSA.BinSyntax.Rewrite
